IRGraphFrames.thy
@@ -168,16 +168,16 @@ lemma elim_inp_set:
   using assms by auto
 
 lemma eval_in_ids:
-  assumes "g m \<turnstile> nid (kind g nid) \<mapsto> v"
+  assumes "g m \<turnstile> (kind g nid) \<mapsto> v"
   shows "nid \<in> ids g"
   using assms by (cases "kind g nid = NoNode"; auto)
 
 (* Main theorem that we want. *)
 theorem stay_same:
   assumes nc: "unchanged (eval_usages g1 nid) g1 g2"
-  assumes g1: "g1 m \<turnstile> nid (kind g1 nid) \<mapsto> v1"
+  assumes g1: "g1 m \<turnstile> (kind g1 nid) \<mapsto> v1"
   assumes wff: "wff_graph g1"
-  shows "g2 m \<turnstile> nid (kind g2 nid) \<mapsto> v1"
+  shows "g2 m \<turnstile> (kind g2 nid) \<mapsto> v1"
 proof -
   have nid: "nid \<in> ids g1"
     using g1 eval_in_ids by simp
@@ -186,24 +186,24 @@ proof -
   then have kind_same: "kind g1 nid = kind g2 nid"
     using nc node_unchanged by blast 
   show ?thesis using g1 nid nc (* kind_same *)
-  proof (induct m nid "(kind g1 nid)" v1 arbitrary: nid rule: "eval.induct")
+  proof (induct m "(kind g1 nid)" v1 arbitrary: nid rule: "eval.induct")
     print_cases
-    case const: (ConstantNode m nid c)
+    case const: (ConstantNode m c)
     then have "(kind g2 nid) = ConstantNode c"
       using kind_unchanged by metis
     then show ?case using eval.ConstantNode const.hyps(1) by metis
   next
-    case param: (ParameterNode val m i nid)
+    case param: (ParameterNode val m i)
     show ?case
-      by (metis eval.ParameterNode kind_unchanged param.hyps(1) param.hyps(2) param.prems(1) param.prems(2))
+      by (metis eval.ParameterNode kind_unchanged param.hyps(1) param.prems(1) param.prems(2))
   next
-    case (ValuePhiNode val m nida uw ux uy nid)
+    case (ValuePhiNode val nida ux uy)
     then have kind: "(kind g2 nid) = ValuePhiNode nida ux uy"
       using kind_unchanged by metis
     then show ?case
       using eval.ValuePhiNode kind ValuePhiNode.hyps(1) by metis 
   next
-    case (ValueProxyNode m child val _ uz nid)
+    case (ValueProxyNode m child val _ nid)
     from ValueProxyNode.prems(1) ValueProxyNode.hyps(3)
     have inp_in: "child \<in> set (inp g1 nid)"
       using child_member_in inputs_of_ValueProxyNode
@@ -212,22 +212,22 @@ proof -
       using wff inp_in_g_wff by blast
     from inp_in have unc: "unchanged (eval_usages g1 child) g1 g2"
       using child_unchanged ValueProxyNode.prems(2) by metis
-    then have "g2 m \<turnstile> child (kind g2 child) \<mapsto> val"
+    then have "g2 m \<turnstile> (kind g2 child) \<mapsto> val"
       using ValueProxyNode.hyps(2) cin
       by blast
     then show ?case
       by (metis ValueProxyNode.hyps(3) ValueProxyNode.prems(1) ValueProxyNode.prems(2) eval.ValueProxyNode kind_unchanged)
   next
-    case (AbsNode m x b v _ nid)
+    case (AbsNode m x b v _)
     then have "unchanged (eval_usages g1 x) g1 g2"
       by (metis child_unchanged elim_inp_set ids_some inputs_of.simps(1) list.set_intros(1))
-    then have "g2 m \<turnstile> x (kind g2 x) \<mapsto> IntVal b v"
+    then have "g2 m \<turnstile> (kind g2 x) \<mapsto> IntVal b v"
       using AbsNode.hyps(1) AbsNode.hyps(2) not_in_g
       by (metis AbsNode.hyps(3) AbsNode.prems(1) elim_inp_set ids_some inp_in_g_wff inputs_of.simps(1) list.set_intros(1) wff)
     then show ?case
       by (metis AbsNode.hyps(3) AbsNode.prems(1) AbsNode.prems(2) eval.AbsNode kind_unchanged)
   next
-    case Node: (NegateNode m x b v _ nid)
+    case Node: (NegateNode m x b v _)
     from inputs_of_NegateNode Node.hyps(3) Node.prems(1) 
     have xinp: "x \<in> set (inp g1 nid)" 
       using child_member_in by (metis member_rec(1))
@@ -235,10 +235,10 @@ proof -
       using wff inp_in_g_wff by blast
     from xinp child_unchanged Node.prems(2)
       have ux: "unchanged (eval_usages g1 x) g1 g2" by blast
-    have x1:"g1 m \<turnstile> x (kind g1 x) \<mapsto> IntVal b v"
+    have x1:"g1 m \<turnstile> (kind g1 x) \<mapsto> IntVal b v"
       using Node.hyps(1) Node.hyps(2)
       by blast
-    have x2: "g2 m \<turnstile> x (kind g2 x) \<mapsto> IntVal b v"
+    have x2: "g2 m \<turnstile> (kind g2 x) \<mapsto> IntVal b v"
       using kind_unchanged ux xin Node.hyps
       by blast
     then show ?case
@@ -248,155 +248,155 @@ proof -
     case node:(AddNode m x b v1 y v2 nid)
     then have ux: "unchanged (eval_usages g1 x) g1 g2"
       by (metis child_unchanged inp.simps inputs_of_AddNode list.set_intros(1))
-    then have x: "g1 m \<turnstile> x (kind g1 x) \<mapsto> IntVal b v1"
+    then have x: "g1 m \<turnstile> (kind g1 x) \<mapsto> IntVal b v1"
       using node.hyps(1) by blast
     have uy: "unchanged (eval_usages g1 y) g1 g2"
       by (metis IRNodes.inputs_of_AddNode child_member_in child_unchanged member_rec(1) node.hyps(5) node.prems(1) node.prems(2))
-    have y: "g1 m \<turnstile> y (kind g1 y) \<mapsto> IntVal b v2"
+    have y: "g1 m \<turnstile> (kind g1 y) \<mapsto> IntVal b v2"
       using node.hyps(3) by blast
     show ?case
       using node.hyps node.prems ux x uy y
       by (metis AddNode inp.simps inp_in_g_wff inputs_of_AddNode kind_unchanged list.set_intros(1) set_subset_Cons subset_iff wff)
   next
-    case node:(SubNode m x b v1 y v2 nid)
+    case node:(SubNode m x b v1 y v2)
     then have ux: "unchanged (eval_usages g1 x) g1 g2"
       by (metis child_member_in child_unchanged inputs_of_SubNode member_rec(1))
-    then have x: "g1 m \<turnstile> x (kind g1 x) \<mapsto> IntVal b v1"
+    then have x: "g1 m \<turnstile> (kind g1 x) \<mapsto> IntVal b v1"
       using node.hyps(1) by blast
     from node have uy: "unchanged (eval_usages g1 y) g1 g2"
       by (metis child_member_in child_unchanged inputs_of_SubNode member_rec(1))
-    have y: "g1 m \<turnstile> y (kind g1 y) \<mapsto> IntVal b v2"
+    have y: "g1 m \<turnstile> (kind g1 y) \<mapsto> IntVal b v2"
       using node.hyps(3) by blast
     show ?case
       using node.hyps node.prems ux x uy y
       by (metis SubNode inp.simps inputs_of_SubNode kind_unchanged list.set_intros(1) set_subset_Cons subsetD wff wff_graph.elims(2))
   next
-    case node:(MulNode m x b v1 y v2 nid)
+    case node:(MulNode m x b v1 y v2)
     then have ux: "unchanged (eval_usages g1 x) g1 g2"
       by (metis child_member_in child_unchanged inputs_of_MulNode member_rec(1))
-    then have x: "g1 m \<turnstile> x (kind g1 x) \<mapsto> IntVal b v1"
+    then have x: "g1 m \<turnstile> (kind g1 x) \<mapsto> IntVal b v1"
       using node.hyps(1) by blast
     from node have uy: "unchanged (eval_usages g1 y) g1 g2"
       by (metis child_member_in child_unchanged inputs_of_MulNode member_rec(1))
-    have y: "g1 m \<turnstile> y (kind g1 y) \<mapsto> IntVal b v2"
+    have y: "g1 m \<turnstile> (kind g1 y) \<mapsto> IntVal b v2"
       using node.hyps(3) by blast
     show ?case
       using node.hyps node.prems ux x uy y
       by (metis MulNode inp.simps inputs_of_MulNode kind_unchanged list.set_intros(1) set_subset_Cons subsetD wff wff_graph.elims(2))
   next
-    case node:(AndNode m x b v1 y v2 nid)
+    case node:(AndNode m x b v1 y v2)
     then have ux: "unchanged (eval_usages g1 x) g1 g2"
       by (metis child_member_in child_unchanged inputs_of_AndNode member_rec(1))
-    then have x: "g1 m \<turnstile> x (kind g1 x) \<mapsto> IntVal b v1"
+    then have x: "g1 m \<turnstile> (kind g1 x) \<mapsto> IntVal b v1"
       using node.hyps(1) by blast
     from node have uy: "unchanged (eval_usages g1 y) g1 g2"
       by (metis child_member_in child_unchanged inputs_of_AndNode member_rec(1))
-    have y: "g1 m \<turnstile> y (kind g1 y) \<mapsto> IntVal b v2"
+    have y: "g1 m \<turnstile> (kind g1 y) \<mapsto> IntVal b v2"
       using node.hyps(3) by blast
     show ?case
       using node.hyps node.prems ux x uy y
       by (metis AndNode inp.simps inputs_of_AndNode kind_unchanged list.set_intros(1) set_subset_Cons subsetD wff wff_graph.elims(2))
   next
-    case node: (OrNode m x b v1 y v2 nid)
+    case node: (OrNode m x b v1 y v2)
     then have ux: "unchanged (eval_usages g1 x) g1 g2"
       by (metis child_member_in child_unchanged inputs_of_OrNode member_rec(1))
-    then have x: "g1 m \<turnstile> x (kind g1 x) \<mapsto> IntVal b v1"
+    then have x: "g1 m \<turnstile> (kind g1 x) \<mapsto> IntVal b v1"
       using node.hyps(1) by blast
     from node have uy: "unchanged (eval_usages g1 y) g1 g2"
       by (metis child_member_in child_unchanged inputs_of_OrNode member_rec(1))
-    have y: "g1 m \<turnstile> y (kind g1 y) \<mapsto> IntVal b v2"
+    have y: "g1 m \<turnstile> (kind g1 y) \<mapsto> IntVal b v2"
       using node.hyps(3) by blast
     show ?case
       using node.hyps node.prems ux x uy y
       by (metis OrNode inp.simps inputs_of_OrNode kind_unchanged list.set_intros(1) set_subset_Cons subsetD wff wff_graph.elims(2))
   next
-    case node: (XorNode m x b v1 y v2 nid)
+    case node: (XorNode m x b v1 y v2)
     then have ux: "unchanged (eval_usages g1 x) g1 g2"
       by (metis child_member_in child_unchanged inputs_of_XorNode member_rec(1))
-    then have x: "g1 m \<turnstile> x (kind g1 x) \<mapsto> IntVal b v1"
+    then have x: "g1 m \<turnstile> (kind g1 x) \<mapsto> IntVal b v1"
       using node.hyps(1) by blast
     from node have uy: "unchanged (eval_usages g1 y) g1 g2"
       by (metis child_member_in child_unchanged inputs_of_XorNode member_rec(1))
-    have y: "g1 m \<turnstile> y (kind g1 y) \<mapsto> IntVal b v2"
+    have y: "g1 m \<turnstile> (kind g1 y) \<mapsto> IntVal b v2"
       using node.hyps(3) by blast
     show ?case
       using node.hyps node.prems ux x uy y
       by (metis XorNode inp.simps inputs_of_XorNode kind_unchanged list.set_intros(1) set_subset_Cons subsetD wff wff_graph.elims(2))
   next
-    case node: (IntegerEqualsNode m x b v1 y v2 val nid)
+    case node: (IntegerEqualsNode m x b v1 y v2 val)
     then have ux: "unchanged (eval_usages g1 x) g1 g2"
       by (metis child_member_in child_unchanged inputs_of_IntegerEqualsNode member_rec(1))
-    then have x: "g1 m \<turnstile> x (kind g1 x) \<mapsto> IntVal b v1"
+    then have x: "g1 m \<turnstile> (kind g1 x) \<mapsto> IntVal b v1"
       using node.hyps(1) by blast
     from node have uy: "unchanged (eval_usages g1 y) g1 g2"
       by (metis child_member_in child_unchanged inputs_of_IntegerEqualsNode member_rec(1))
-    have y: "g1 m \<turnstile> y (kind g1 y) \<mapsto> IntVal b v2"
+    have y: "g1 m \<turnstile> (kind g1 y) \<mapsto> IntVal b v2"
       using node.hyps(3) by blast
     show ?case
       using node.hyps node.prems ux x uy y
       by (metis (full_types) IntegerEqualsNode child_member_in in_set_member inputs_of_IntegerEqualsNode kind_unchanged list.set_intros(1) set_subset_Cons subsetD wff wff_graph.elims(2))
   next
-    case node: (IntegerLessThanNode m x b v1 y v2 val nid)
+    case node: (IntegerLessThanNode m x b v1 y v2 val)
     then have ux: "unchanged (eval_usages g1 x) g1 g2"
       by (metis child_member_in child_unchanged inputs_of_IntegerLessThanNode member_rec(1))
-    then have x: "g1 m \<turnstile> x (kind g1 x) \<mapsto> IntVal b v1"
+    then have x: "g1 m \<turnstile> (kind g1 x) \<mapsto> IntVal b v1"
       using node.hyps(1) by blast
     from node have uy: "unchanged (eval_usages g1 y) g1 g2"
       by (metis child_member_in child_unchanged inputs_of_IntegerLessThanNode member_rec(1))
-    have y: "g1 m \<turnstile> y (kind g1 y) \<mapsto> IntVal b v2"
+    have y: "g1 m \<turnstile> (kind g1 y) \<mapsto> IntVal b v2"
       using node.hyps(3) by blast
     show ?case
       using node.hyps node.prems ux x uy y
       by (metis (full_types) IntegerLessThanNode child_member_in in_set_member inputs_of_IntegerLessThanNode kind_unchanged list.set_intros(1) set_subset_Cons subsetD wff wff_graph.elims(2))
   next
-    case node: (ShortCircuitOrNode m x b v1 y v2 val nid)
+    case node: (ShortCircuitOrNode m x b v1 y v2 val)
     then have ux: "unchanged (eval_usages g1 x) g1 g2"
       by (metis child_member_in child_unchanged inputs_of_ShortCircuitOrNode member_rec(1))
-    then have x: "g1 m \<turnstile> x (kind g1 x) \<mapsto> IntVal b v1"
+    then have x: "g1 m \<turnstile> (kind g1 x) \<mapsto> IntVal b v1"
       using node.hyps(1) by blast
     from node have uy: "unchanged (eval_usages g1 y) g1 g2"
       by (metis child_member_in child_unchanged inputs_of_ShortCircuitOrNode member_rec(1))
-    have y: "g1 m \<turnstile> y (kind g1 y) \<mapsto> IntVal b v2"
+    have y: "g1 m \<turnstile> (kind g1 y) \<mapsto> IntVal b v2"
       using node.hyps(3) by blast
-    have x2: "g2 m \<turnstile> x (kind g2 x) \<mapsto> IntVal b v1"
+    have x2: "g2 m \<turnstile> (kind g2 x) \<mapsto> IntVal b v1"
       by (metis inp.simps inputs_of_ShortCircuitOrNode list.set_intros(1) node.hyps(2) node.hyps(6) node.prems(1) subsetD ux wff wff_graph.elims(2))
-    have y2: "g2 m \<turnstile> y (kind g2 y) \<mapsto> IntVal b v2"
+    have y2: "g2 m \<turnstile> (kind g2 y) \<mapsto> IntVal b v2"
       by (metis basic_trans_rules(31) inp.simps inputs_of_ShortCircuitOrNode list.set_intros(1) node.hyps(4) node.hyps(6) node.prems(1) set_subset_Cons uy wff wff_graph.elims(2))
     show ?case
       using node.hyps node.prems ux x uy y x2 y2
       by (metis ShortCircuitOrNode kind_unchanged)
   next
-    case node: (LogicNegationNode m x b v1 val nida nid)
+    case node: (LogicNegationNode m x b v1 val nida)
     then have ux: "unchanged (eval_usages g1 x) g1 g2"
       by (metis child_member_in child_unchanged inputs_of_LogicNegationNode member_rec(1))
-    then have x:"g2 m \<turnstile> x (kind g2 x) \<mapsto> IntVal b v1"
+    then have x:"g2 m \<turnstile> (kind g2 x) \<mapsto> IntVal b v1"
       by (metis inp.simps inp_in_g_wff inputs_of_LogicNegationNode list.set_intros(1) node.hyps(2) node.hyps(4) wff)
     then show ?case
       by (metis LogicNegationNode kind_unchanged node.hyps(3) node.hyps(4) node.prems(1) node.prems(2))
   next
-    case node:(ConditionalNode m condition cond trueExp b trueVal falseExp falseVal val nid)
+    case node:(ConditionalNode m condition cond trueExp b trueVal falseExp falseVal val)
     have c: "condition \<in> set(inp g1 nid)"
       by (metis IRNodes.inputs_of_ConditionalNode child_member_in member_rec(1) node.hyps(8) node.prems(1))
     then have "unchanged (eval_usages g1 condition) g1 g2"
       using child_unchanged node.prems(2) by blast
-    then have cond: "g2 m \<turnstile> condition (kind g2 condition) \<mapsto> IntVal 1 cond"
+    then have cond: "g2 m \<turnstile> (kind g2 condition) \<mapsto> IntVal 1 cond"
       using node c inp_in_g_wff wff by blast
 
     have t: "trueExp \<in> set(inp g1 nid)"
       by (metis IRNodes.inputs_of_ConditionalNode child_member_in member_rec(1) node.hyps(8) node.prems(1))
     then have utrue: "unchanged (eval_usages g1 trueExp) g1 g2"
       using node.prems(2) child_unchanged by blast
-    then have trueVal: "g2 m \<turnstile> trueExp (kind g2 trueExp) \<mapsto> IntVal b (trueVal)"
+    then have trueVal: "g2 m \<turnstile> (kind g2 trueExp) \<mapsto> IntVal b (trueVal)"
       using node.hyps node t inp_in_g_wff wff by blast
 
     have f: "falseExp \<in> set(inp g1 nid)"
       by (metis IRNodes.inputs_of_ConditionalNode child_member_in member_rec(1) node.hyps(8) node.prems(1))
     then have ufalse: "unchanged (eval_usages g1 falseExp) g1 g2"
       using node.prems(2) child_unchanged by blast
-    then have falseVal: "g2 m \<turnstile> falseExp (kind g2 falseExp) \<mapsto> IntVal b (falseVal)"
+    then have falseVal: "g2 m \<turnstile> (kind g2 falseExp) \<mapsto> IntVal b (falseVal)"
       using node.hyps node f inp_in_g_wff wff by blast
 
-    have "g2 m \<turnstile> nid (kind g2 nid) \<mapsto> val"
+    have "g2 m \<turnstile> (kind g2 nid) \<mapsto> val"
       using kind_same trueVal falseVal cond
       by (metis ConditionalNode kind_unchanged node.hyps(7) node.hyps(8) node.prems(1) node.prems(2))
     then show ?case
@@ -406,28 +406,28 @@ proof -
     case (RefNode m x val nid)
     have x: "x \<in> set(inp g1 nid)"
       by (metis IRNodes.inputs_of_RefNode RefNode.hyps(3) RefNode.prems(1) child_member_in member_rec(1))
-    then have ref: "g2 m \<turnstile> x (kind g2 x) \<mapsto> val"
+    then have ref: "g2 m \<turnstile> (kind g2 x) \<mapsto> val"
       using RefNode.hyps(2) RefNode.prems(2) child_unchanged inp_in_g_wff wff by blast
     then show ?case
       by (metis RefNode.hyps(3) RefNode.prems(1) RefNode.prems(2) eval.RefNode kind_unchanged)
   next
-    case (InvokeNodeEval val m nida _ callTarget classInit stateDuring stateAfter nex)
+    case (InvokeNodeEval val m _ callTarget classInit stateDuring stateAfter nex)
     then show ?case
       by (metis eval.InvokeNodeEval kind_unchanged)
   next
-    case (SignedDivNode m x b v1 y v2 nid zeroCheck frameState nex)
+    case (SignedDivNode m x b v1 y v2 zeroCheck frameState nex)
     have xinp: "x \<in> set(inp g1 nid)"
       by (metis IRNodes.inputs_of_SignedDivNode SignedDivNode.hyps(5) SignedDivNode.prems(1) append_Cons child_member_in member_rec(1))
-    from xinp have x: "g2 m \<turnstile> x (kind g2 x) \<mapsto> IntVal b v1"
+    from xinp have x: "g2 m \<turnstile> (kind g2 x) \<mapsto> IntVal b v1"
       using SignedDivNode child_unchanged inp_in_g_wff wff by blast
     have yinp: "y \<in> set(inp g1 nid)"
       by (metis IRNodes.inputs_of_SignedDivNode SignedDivNode.hyps(5) SignedDivNode.prems(1) append_Cons child_member_in member_rec(1))
-    from yinp have y: "g2 m \<turnstile> y (kind g2 y) \<mapsto> IntVal b v2"
+    from yinp have y: "g2 m \<turnstile> (kind g2 y) \<mapsto> IntVal b v2"
       using SignedDivNode child_unchanged inp_in_g_wff wff by blast
     from x y show ?case
       by (metis SignedDivNode.hyps(5) SignedDivNode.prems(1) SignedDivNode.prems(2) eval.SignedDivNode kind_unchanged)
   next
-    case (InvokeWithExceptionNodeEval val m nida _ callTarget classInit stateDuring stateAfter nex exceptionEdge)
+    case (InvokeWithExceptionNodeEval val m _ callTarget classInit stateDuring stateAfter nex exceptionEdge)
     then show ?case
       by (metis eval.InvokeWithExceptionNodeEval kind_unchanged)
   next
@@ -438,7 +438,7 @@ proof -
     case (IsNullNode m obj ref val)
     have obj: "obj \<in> set(inp g1 nid)"
       by (metis IRNodes.inputs_of_IsNullNode IsNullNode.hyps(4) inp.simps list.set_intros(1))
-    then have ref: "g2 m \<turnstile> obj (kind g2 obj) \<mapsto> ObjRef ref"
+    then have ref: "g2 m \<turnstile> (kind g2 obj) \<mapsto> ObjRef ref"
       using IsNullNode.hyps(1) IsNullNode.hyps(2) IsNullNode.prems(2) child_unchanged eval_in_ids by blast
     then show ?case
       by (metis (full_types) IsNullNode.hyps(3) IsNullNode.hyps(4) IsNullNode.prems(1) IsNullNode.prems(2) eval.IsNullNode kind_unchanged)
@@ -451,7 +451,7 @@ proof -
     have object: "object \<in> set(inp g1 nid)"
       using inputs_of_PiNode inp.simps
       by (metis PiNode.hyps(3) append_Cons list.set_intros(1))
-    then have ref: "g2 m \<turnstile> object (kind g2 object) \<mapsto> val"
+    then have ref: "g2 m \<turnstile> (kind g2 object) \<mapsto> val"
       using PiNode.hyps(1) PiNode.hyps(2) PiNode.prems(2) child_unchanged eval_in_ids by blast
     then show ?case
       by (metis PiNode.hyps(3) PiNode.prems(1) PiNode.prems(2) eval.PiNode kind_unchanged)
